shift-reset/core/record.v
@@ -12,10 +12,10 @@ Fixpoint record_lookup (l : ident) (r : record) : option val :=
   | RecordCons l' v r' => if ident_eqb l l' then Some v else record_lookup l r'
   end.
 
-Fixpoint record_lookup_remove (l : ident) (r : record) : option val * record :=
+Fixpoint record_lookup_delete (l : ident) (r : record) : option val * record :=
   match r with
   | RecordNil => (None, r)
   | RecordCons l' v r' =>
       if ident_eqb l l' then (Some v, r')
-      else let (o, r') := record_lookup_remove l r' in (o, RecordCons l' v r')
+      else let (o, r') := record_lookup_delete l r' in (o, RecordCons l' v r')
   end.
